symprec.v
@@ -1,0 +1,593 @@
+Require Import Coq.Logic.Decidable.
+Require Import PeanoNat.
+Require Import Coq.Strings.String.
+Require Import Ascii.
+Require Import Bool.
+Require Import Nat.
+Require Import Lia.
+
+Require Import LIR.maps.
+Require Import LIR.lir.
+Require Import LIR.precision.
+
+Set Implicit Arguments.
+
+
+Inductive PrecMem : Mem -> Mem -> Prop :=
+| PrecMemE : PrecMem EmptyMem EmptyMem
+| PrecMemUD : forall addr idx v1 v2 m1 m2,
+    Value v1 ->
+    Value v2 ->
+    Precision PEmpty v1 IRTStar v2 IRTStar ->
+    PrecMem m1 m2 ->
+    PrecMem (Update addr idx v1 m1) (Update addr idx v2 m2)
+.
+
+
+Infix "<M|" := PrecMem (at level 80).
+
+
+Lemma PrecCorrect1 : forall m1 m2, m1 <M| m2 -> mem_correct m1.
+Proof.
+  unfold mem_correct.
+  intros * H.
+  induction H; intros *; simpl.
+  - eauto using Value, IRTyping.
+  - breakIndexDec; subst; eauto using PrecisionType1Empty.
+Qed.
+
+
+Lemma PrecCorrect2 : forall m1 m2, m1 <M| m2 -> mem_correct m2.
+Proof.
+  unfold mem_correct.
+  intros * H.
+  induction H; intros *; simpl.
+  - eauto using Value, IRTyping.
+  - breakIndexDec; subst; eauto using PrecisionType2Empty.
+Qed.
+
+
+Lemma PrecFreshaux : forall m1 m2,
+    m1 <M| m2 -> freshaux m1 = freshaux m2.
+Proof.
+  intros * HOM.
+  induction HOM; simpl; eauto.
+Qed.
+
+
+Lemma PrecFresh : forall m1 m2 free m1', 
+    m1 <M| m2 ->
+    (free, m1') = fresh m1 ->
+    exists m2', m1' <M| m2' /\ (free, m2') = fresh m2.
+Proof.
+  unfold fresh.
+  intros * HOM HF.
+  injection HF; intros; subst; clear HF.
+  replace (freshaux m2) with (freshaux m1) by auto using PrecFreshaux.
+  eexists. split; only 2: trivial;
+  eauto 6 using PrecMem, Value, Precision.
+Qed.
+
+
+Axiom PrecIndex : forall e1 e2,
+    Precision PEmpty e1 IRTStar e2 IRTStar ->
+    ToIndex e1 = ToIndex e2.
+
+
+Lemma PrecQuery : forall m1 m2 a i1 i2,
+    m1 <M| m2 ->
+    Precision PEmpty i1 IRTStar i2 IRTStar ->
+    Precision PEmpty (query a i1 m1) IRTStar (query a i2 m2) IRTStar.
+Proof.
+  intros * HOM HP.
+  induction HOM; simpl.
+  - eauto using Precision.
+  - rewrite <- (PrecIndex HP).
+    breakIndexDec; trivial.
+Qed.
+
+
+Lemma PrecUpdate : forall m1 m2 a i1 i2 v1 v2,
+    m1 <M| m2 ->
+    Value v1 ->
+    Value v2 ->
+    Precision PEmpty i1 IRTStar i2 IRTStar ->
+    Precision PEmpty v1 IRTStar v2 IRTStar ->
+    Update a (ToIndex i1) v1 m1 <M| Update a (ToIndex i2) v2 m2.
+Proof.
+  intros * HOM HV1 HV2 HP1 HP2.
+  rewrite <- (PrecIndex HP1).
+  auto using PrecMem.
+Qed.
+
+
+(*
+Lemma subst_typing : forall e2 Γ var tv te e1,
+  var |=> tv; Γ |= e2 : te -> MEmpty |= e1 : tv ->
+       Γ |= ([var := e1] e2) : te.
+Proof.
+  induction e2; intros Γ var tv te e1 HT2 HT1;
+  simpl; inversion HT2; subst;
+  breakStrDec;
+  eauto 6 using inclusion_typing, inclusion_shadow, inclusion_permute,
+    IRTyping, typing_empty, InNotEq.
+  - assert (te = tv). { rewrite InEq in H1. congruence. }
+      subst. eauto using typing_empty.
+Qed.
+*)
+
+
+Lemma InInclusionNE : forall (Γ Γ' : IREnvironment) var var' t t1,
+    inclusion (var |=> t1; Γ') Γ ->
+    var <> var' ->
+    In Γ var' = Some t ->
+    In Γ' var' = Some t.
+Admitted.
+
+
+Lemma PrecSubs : forall body Γ Γ' var  body' v1 v2 t1 t2 t1' t2'
+                        (H12: t1 <| t2),
+    Precision PEmpty v1 t1 v2 t2 ->
+    PEEquiv (ExpandPEnv Γ var t1 t2 H12) Γ' ->
+    Precision Γ' body t1' body' t2' ->
+    Precision Γ ([var := v1] body) t1' ([var := v2] body') t2'.
+Proof.
+  intros * HPV HPE HPB.
+  generalize dependent Γ.
+  induction HPB; intros ? HPE; eauto using Precision.
+
+  - simpl.
+    breakStrDec.
+    + destruct Γ. destruct Γ0. simpl in H. simpl in H0.
+      inversion HPE; subst.
+      apply InEq' in H.
+      apply InEq' in H0.
+      subst.
+      eauto using PrecisionInclusion, PinclusionEmpty.
+    + destruct Γ. destruct Γ0. simpl in H. simpl in H0.
+      inversion HPE; subst. 
+       eapply PVar; simpl; eauto using InNotEq.
+
+  - simpl.
+    breakStrDec.
+    + apply PFun with (H12 := H0).
+
+    +
+
+Precision (ExpandPEnv Γ var0 t0 t3 H0) d1 t1' d2 t2'
+
+
+(*    + 
+      eauto using Precision.
+    + eapply PFun with (H12 := H0).
+      eapply IHHPB.
+      unfold Pinclusion in HPI. destruct HPI.
+      unfold Pinclusion. split.
+
+      assert (Pinclusion
+               (ExpandPEnv (ExpandPEnv Γ0 var0 t0 t3 H0) var t1 t2 H12)
+               (ExpandPEnv Γ var0 t0 t3 H0)). {
+        destruct Γ0.
+        destruct Γ.
+        rewrite Expand1 in i.
+        rewrite Expand2 in i0.
+        unfold Pinclusion. split.
+*)
+Admitted.
+
+
+Lemma PrecSubs' : forall var t1 t2 t1' t2' body body' v1 v2,
+    Precision PEmpty (IREFun var t1 body) (IRTFun t1 t1')
+                     (IREFun var t2 body') (IRTFun t2 t2') ->
+    Precision PEmpty v1 t1 v2 t2 ->
+    Precision PEmpty ([var := v1] body) t1' ([var := v2] body') t2'.
+Proof.
+  intros * HPF HPV.
+  inversion HPF; subst.
+  eapply PrecSubs; eauto.
+  unfold Pinclusion; split.
+  * unfold inclusion.
+    rewrite Expand1.
+    rewrite Expand1.
+    trivial.
+  * unfold inclusion.
+    rewrite Expand2.
+    rewrite Expand2.
+    trivial.
+
+  Unshelve. trivial.
+Qed.
+
+
+Lemma GroundFlat' : forall t g g',
+    t <| Tag2Type g' -> t = Tag2Type g -> g = g'.
+Proof.
+  intros * H HEq. subst. auto using GroundFlat.
+Qed.
+
+
+Ltac ContraTags :=
+  try match goal with
+    [H: IRTStar <| Tag2Type _ |- _] =>
+      apply NoneBiggerThanStar in H
+  end;
+  try match goal with
+    [H: IRTStar = Tag2Type ?g |- _] =>
+      destruct g; discriminate
+  end.
+
+
+Lemma GroundType: forall g t g',
+    t <| Tag2Type g -> Type2Tag t = Some g' -> g = g'.
+Proof.
+  intros * HT Heq.
+  destruct t eqn:Heq';
+  ContraTags;
+  try (injection Heq; intros;
+    rewrite <- Heq' in HT;
+    replace t with (Tag2Type g') in HT by (subst; trivial);
+    symmetry;
+    eauto using GroundFlat).
+  injection Heq; intros; subst.
+  assert (IRTFun i1 i2 <| Tag2Type TgFun) by (simpl; auto using TPrecision).
+  eauto using GroundTop.
+Qed.
+
+
+Lemma stepValueMem : forall e1 e2 e2' t1 t2 m m',
+    Precision PEmpty e1 t1 e2 t2 ->
+    Value e1 ->
+    m / e2 --> m' / e2' -> m = m'.
+Proof.
+  intros * HP HV HStep.
+  remember PEmpty as Γ.
+  generalize dependent m'.
+  generalize dependent m.
+  generalize dependent e2'.
+  induction HP; intros * HStep; inversion HV;
+  inversion HStep; subst; eauto using Precision.
+Qed.
+
+
+Lemma PrecisionPreservation : forall e1 e2 e2' t1 t2 m m',
+    Precision PEmpty e1 t1 e2 t2 ->
+    Value e1 ->
+    m / e2 --> m' / e2' ->
+    Precision PEmpty e1 t1 e2' t2.
+Proof.
+  intros * HP HV HStep.
+  remember PEmpty as Γ.
+  generalize dependent m'.
+  generalize dependent m.
+  generalize dependent e2'.
+  induction HP; intros * HStep; inversion HV; subst;
+  inversion HStep; subst; eauto using Precision;
+  inversion HStep; subst;
+  try (inversion H5;
+       inversion HP; subst; trivial).
+  - inversion H6.
+  - inversion HP; subst; trivial.
+    ContraTags.
+Qed.
+
+
+Lemma PrecisionPreservationM : forall e1 e2 e2' t1 t2 m m',
+    Precision PEmpty e1 t1 e2 t2 ->
+    Value e1 ->
+    m / e2 -->* m' / e2' ->
+    Precision PEmpty e1 t1 e2' t2.
+Proof.
+  intros * HP HV HStep.
+  induction HStep; eauto using PrecisionPreservation.
+Qed.
+
+
+Lemma BoxPreservePrecision : forall e m m' b tg v t,
+  m / IREBox tg e -->* m' / b ->
+  Precision PEmpty v t (IREBox tg e) IRTStar ->
+  Value v ->
+  exists o, b = IREBox tg o /\ Precision PEmpty v t b IRTStar.
+Proof.
+  intros * Hst.
+  remember (IREBox tg e) as E.
+  generalize dependent e.
+  induction Hst; intros * HEq HP HV.
+  - exists e0. auto.
+  - subst.
+    replace m' with m in * by (eapply stepValueMem; eauto).
+    inversion H; subst.
+    eauto using PrecisionPreservation.
+Qed.
+
+
+Lemma ValueStarP : forall tg t v e m e',
+    Precision PEmpty v t e IRTStar ->
+    t <| Tag2Type tg ->
+    Value v ->
+    m / e -->* m / e' ->
+    Value e' ->
+      exists o,
+        e' = IREBox tg o /\ Precision PEmpty v t e' IRTStar.
+Proof.
+  intros * HP HSty HVP HStep HV.
+  inversion HP; subst; try (inversion HVP; fail); 
+  ContraTags.
+  replace g with tg in *. 2:{
+    apply PPT in H.
+    eauto using GroundTop.
+  }
+  eauto using BoxPreservePrecision.
+Qed.
+
+
+Lemma ValueLR : forall e1 t1 e2 t2 m,
+  Precision PEmpty e1 t1 e2 t2 ->
+  Value e1 ->
+  exists e2', m / e2 -->* m / e2' /\ Value e2'.
+Proof.
+  intros * HP HV.
+  remember PEmpty as Γ eqn:Heq.
+  induction HP; subst Γ; inversion HV; subst;
+  (* instanciate and break induction hypothesis *)
+  try match goal with
+  [IH: _ -> Value ?E -> _ ,
+   HV: Value ?E |- _] =>
+     specialize (IH eq_refl HV) as [? [? ?]]
+  end;
+  try (eexists; split; eauto using MStRefl, Value; fail);
+  try (eexists; split; eauto using CongBox, Value; fail);
+
+  pose proof HP as HP';
+  apply PrecisionType1 in HP';
+  inversion HP'; subst; clear HP';
+  ContraTags;
+
+  specialize (ValueStarP _ HP H HV H0 H1) as [? [? _]];
+      subst;
+
+  try (eapply GroundType in H; only 2: (simpl; trivial);
+    apply valBoxVal in H1;
+    exists x0; split;
+    eauto using multiTrans, CongUnbox, step, multistep). 
+Qed.
+
+
+Ltac BreakIH :=
+  match goal with
+    [IH: context [_ / ?E --> _ / _ -> (PrecMem _ _) -> _] ,
+     HSt: ?M / ?E --> _ / _ ,
+     HM: ?M <M| ?M' |- _ ] => idtac E M M';
+       specialize (IH eq_refl _ _ _ _ HSt HM) as [? [? [? [? ?]]]]
+  end.
+
+
+Lemma NoValueUnbox : forall tg e (C : Type), 
+    Value (IREUnbox tg e) -> C.
+Proof.
+  intros * H.
+  exfalso.
+  inversion H.
+Qed.
+
+
+Ltac NoValueUnbox :=
+  match goal with [H: Value (IREUnbox _ _) |- _] =>
+    eapply NoValueUnbox; eauto
+  end.
+
+
+Theorem Sym : forall m1 e1 t1 e2 m2 t2 m1' e1', 
+  Precision PEmpty e1 t1 e2 t2 ->
+  m1 / e1 --> m1' / e1'   ->
+  m1 <M| m2 ->
+  exists e2' m2',
+    m2 / e2 -->* m2' / e2' /\ m1' <M| m2' /\ Precision PEmpty e1' t1 e2' t2.
+Proof.
+  intros * HP.
+  generalize dependent m2.
+  generalize dependent e1'.
+  generalize dependent m1'.
+  generalize dependent m1.
+  remember PEmpty as Γ.
+  induction HP; intros * Hstep HM; try (inversion Hstep; fail).
+
+  - (* Plus *)
+    inversion Hstep; subst.
+
+    + (* StPlus1 *)
+      BreakIH.
+      eexists; eexists; split; try split; eauto using Precision, CongPlus1.
+
+    + (* StPlus2 *)
+      BreakIH.
+      specialize (ValueLR m2 HP1 H2) as [? [? ?]].
+      eexists; exists x0; split; try split;
+        eauto using multiTrans, CongPlus1, CongPlus2,
+                    Precision, PrecisionPreservationM.
+
+    + (* StPlus *)
+      clear IHHP1 IHHP2.
+      specialize (ValueLR m2 HP1 (Vnum n1)) as [? [? ?]].
+      specialize (ValueLR m2 HP2 (Vnum n2)) as [? [? ?]].
+
+      assert (N1: x = IRENum n1). {
+        specialize (PrecisionPreservationM HP1 (Vnum n1) H) as NH1.
+        inversion NH1; subst; trivial; NoValueUnbox.
+      }
+
+      assert (N2: x0 = IRENum n2). {
+        specialize (PrecisionPreservationM HP2 (Vnum n2) H1) as NH2.
+        inversion NH2; subst; trivial; NoValueUnbox.
+      }
+
+      subst.
+      exists (IRENum (n1 + n2)). exists m2. split; try split;
+        eauto 7 using multiTrans, CongPlus1, CongPlus2, multistep1, step,
+           Precision.
+
+
+  - (* StCstr *)
+    inversion Hstep; subst.
+    specialize (PrecFresh HM H) as [? [? ?]].
+    eexists; eexists; split; try split;
+    eauto using multistep1, step, Precision.
+
+
+  - (* Get *)
+    inversion Hstep; subst.
+
+    + (* StGet1 *)
+      BreakIH.
+      eexists; eexists; split; try split; eauto using Precision, CongGet1.
+
+    + (* StGet2 *)
+      BreakIH.
+      specialize (ValueLR m2 HP1 H2) as [? [? ?]].
+      eexists; exists x0; split; try split;
+        eauto using multiTrans, CongGet1, CongGet2,
+                    Precision, PrecisionPreservationM.
+
+    + (* StGet *)
+      clear IHHP1 IHHP2.
+
+      specialize (ValueLR m2 HP1 (Vtbl a)) as [? [? ?]].
+      specialize (ValueLR m2 HP2 H4) as [? [? ?]].
+
+      assert (N1: x = IREAddr a). {
+        specialize (PrecisionPreservationM HP1 (Vtbl a) H) as NH1.
+        inversion NH1; subst; trivial; NoValueUnbox.
+      } subst.
+
+      exists (query a x0 m2). exists m2. split; try split;
+        eauto 7 using multiTrans, CongGet1, CongGet2, multistep1, step,
+           Precision, PrecQuery, PrecisionPreservationM.
+
+  - (* Set *)
+    inversion Hstep; subst.
+
+    + (* StSet1 *)
+      BreakIH.
+      eexists; eexists; split; try split; eauto using Precision, CongSet1.
+
+    + (* StSet2 *)
+      BreakIH.
+      specialize (ValueLR m2 HP1 H5) as [? [? ?]].
+      eexists; exists x0; split; try split;
+        eauto using multiTrans, CongSet1, CongSet2,
+                    Precision, PrecisionPreservationM.
+
+    + (* StSet3 *)
+      BreakIH.
+      specialize (ValueLR m2 HP1 H3) as [? [? ?]].
+      specialize (ValueLR m2 HP2 H6) as [? [? ?]].
+      eexists; exists x0; split; try split;
+        eauto 6 using multiTrans, CongSet1, CongSet2, CongSet3,
+                    Precision, PrecisionPreservationM.
+
+    + (* StSet *)
+      clear IHHP1 IHHP2 IHHP3.
+
+      specialize (ValueLR m2 HP1 (Vtbl a)) as [? [? ?]].
+      specialize (ValueLR m2 HP2 H5) as [? [? ?]].
+      specialize (ValueLR m2 HP3 H6) as [? [? ?]].
+
+      assert (N1: x = IREAddr a). {
+        specialize (PrecisionPreservationM HP1 (Vtbl a) H) as NH1.
+        inversion NH1; subst; trivial; NoValueUnbox.
+      } subst.
+
+      exists x1. exists (Update a x0 x1 m2). split; try split;
+        eauto 10 using multiTrans, CongSet1, CongSet2, CongSet3,
+          multistep1, step, Precision, PrecQuery, PrecisionPreservationM,
+          PrecUpdate.
+
+
+  - (* StFunApp *)
+    inversion Hstep; subst.
+
+    + (* StFunApp1 *)
+      BreakIH.
+      eexists; eexists; split; try split; eauto using Precision, CongFunApp1.
+
+    + (* StFunApp2 *)
+      BreakIH.
+      specialize (ValueLR m2 HP2 H2) as [? [? ?]].
+      eexists; exists x0; split; try split;
+        eauto using multiTrans, CongFunApp1, CongFunApp2,
+                    Precision, PrecisionPreservationM.
+
+    + (* StFunApp *)
+      clear IHHP1 IHHP2.
+
+      replace t with t1 in * by 
+        (apply PrecisionType1 in HP2; inversion HP2; subst; trivial).
+
+      specialize (ValueLR m2 HP1 H4) as [? [? ?]].
+      specialize (ValueLR m2 HP2 (Vfun var t1 body)) as [? [? ?]].
+
+      assert (N1: exists body', x0 = IREFun var t2 body'). {
+        specialize (PrecisionPreservationM HP2 (Vfun var t1 body) H1) as NH1.
+        inversion NH1; subst; eauto; NoValueUnbox.
+      }
+      destruct N1 as [body' ?].
+      subst.
+      exists ([var := x] body'). exists m2. split; try split;
+        eauto 7 using multiTrans, CongFunApp1, CongFunApp2, multistep1, step,
+           Precision.
+
+      eauto using PrecSubs', PrecisionPreservationM, Value.
+
+  - (* BoxR *)
+      subst.
+      BreakIH.
+      eexists; eexists; split; try split; eauto using Precision, CongBox.
+
+  - (* BoxL *)
+      inversion Hstep; subst.
+      BreakIH.
+      eexists; eexists; split; try split; eauto using Precision, CongBox.
+
+  - (* UnboxL *)
+      inversion Hstep; subst.
+
+      + BreakIH.
+       eexists; eexists; split; try split; eauto using Precision, CongUnbox.
+
+      + clear IHHP.
+        specialize (ValueLR m2 HP (Vbox g e1' H5)) as [? [? ?]].
+
+        inversion HP; subst; ContraTags.
+        * exfalso. apply PPT in H1. ContraTags.
+        * specialize (@ValueStarP _ _ _ _ _ _ H3 (TPrecisionRefl (Tag2Type g))
+            H5 H H0) as [? [? ?]].
+          subst.
+          eexists; eexists; split; try split; eauto.
+
+  - (* UnboxR *)
+      subst.
+      BreakIH.
+      eexists; eexists; split; try split; eauto using Precision, CongUnbox.
+Qed.
+
+
+
+(*
+Lemma BoxPreserveType : forall e m m' b tg,
+  m / IREBox tg e -->* m' / b ->
+  MEmpty |= e : Tag2Type tg ->
+  mem_correct m ->
+  exists o, b = IREBox tg o /\ MEmpty |= o : Tag2Type tg.
+Proof.
+  intros * HSt.
+  remember (IREBox tg e) as E.
+  generalize dependent tg.
+  generalize dependent e.
+  induction HSt; intros; subst e.
+  - exists e0; split; trivial.
+  - inversion H; subst.
+    specialize (PresTy _ _ _ _ _ H1 H0 H7) as HTy.
+    specialize (PresMC _ _ _ _ _ H1 H0 H7) as HM'.
+    specialize (IHHSt _ _ eq_refl HTy HM') as [? [? ?]].
+    exists x; split; trivial.
+Qed.
+*)
