makefile
@@ -4,9 +4,10 @@ lir.vo: lir.v
 	coqc -Q . LIR $<
 
 
-lir.vo: maps.vo
-dyn.vo: maps.vo lir.vo
-precision.vo: maps.vo lir.vo dyn.vo
-pallene.vo: maps.vo lir.vo
-lua.vo: maps.vo pallene.vo lir.vo dyn.vo
+lir.vo: lir.v maps.vo
+dyn.vo: dyn.v maps.vo lir.vo
+precision.vo: precision.v maps.vo lir.vo dyn.vo
+symprec.vo: symprec.v precision.vo maps.vo lir.vo
+pallene.vo: pallene.v maps.vo lir.vo
+lua.vo: lua.v maps.vo pallene.vo lir.vo dyn.vo
 
